row equivalence and elaboration soundness without Monotype_open_preservation

TabularTypeInterpreter/F⊗⊕ω/Lemmas/Type.lean
@@ -1,10 +1,23 @@
 import Aesop
+import TabularTypeInterpreter.«F⊗⊕ω».Lemmas.Environment.Basic
 import TabularTypeInterpreter.«F⊗⊕ω».Semantics.Environment
 import TabularTypeInterpreter.«F⊗⊕ω».Semantics.Type
 
 namespace TabularTypeInterpreter.«F⊗⊕ω»
 
 namespace «Type»
+
+@[elab_as_elim]
+def rec_uniform {motive : «Type» → Prop} (var : ∀ a : TypeVar, motive (var a))
+  (lam : ∀ K A, motive A → motive (lam K A)) (app : ∀ A B, motive A → motive B → motive (app A B))
+  («forall» : ∀ K A, motive A → motive («forall» K A))
+  (arr : ∀ A B, motive A → motive B → motive (arr A B))
+  (list : ∀ As, (∀ A ∈ As, motive A) → motive (list As))
+  (listApp : ∀ A B, motive A → motive B → motive (listApp A B))
+  (prod : ∀ A, motive A → motive (prod A)) (sum : ∀ A, motive A → motive (sum A)) (A : «Type»)
+  : motive A :=
+  rec (motive_1 := motive) var lam app «forall» arr list listApp prod sum (fun _ => (nomatch ·))
+    (fun _ _ ih₀ ih₁ _ mem => match mem with | .head _ => ih₀ | .tail _ mem' => ih₁ _ mem') A
 
 @[simp]
 theorem TypeVar_open_sizeOf (A : «Type») : sizeOf (A.TypeVar_open a n) = sizeOf A := by
@@ -82,6 +95,13 @@ theorem TypeVar_open_sizeOf (A : «Type») : sizeOf (A.TypeVar_open a n) = sizeO
 where
   rev : ∀ a : «Type», a._sizeOf_1 = sizeOf a := fun _ => by dsimp only [sizeOf]
 
+theorem TypeVar_open_comm (A : «Type»)
+  : m ≠ n → (A.TypeVar_open a m).TypeVar_open a' n = (A.TypeVar_open a' n).TypeVar_open a m := by
+  induction A using rec_uniform generalizing m n <;> aesop (add simp TypeVar_open)
+
+theorem TypeVar_open_eq_Type_open_var : TypeVar_open A a n = A.Type_open (.var a) n := by
+  induction A using rec_uniform generalizing n <;> aesop (add simp [TypeVar_open, Type_open])
+
 namespace TypeVarLocallyClosed
 
 theorem weaken {A : «Type»} : A.TypeVarLocallyClosed m → A.TypeVarLocallyClosed (m + n)
@@ -101,6 +121,70 @@ theorem weaken {A : «Type»} : A.TypeVarLocallyClosed m → A.TypeVarLocallyClo
   | listApp A'lc Blc => listApp A'lc.weaken Blc.weaken
   | prod A'lc => prod A'lc.weaken
   | sum A'lc => sum A'lc.weaken
+
+theorem Type_open_drop (h : m < n) (Aoplc : (Type_open A B m).TypeVarLocallyClosed n)
+  : A.TypeVarLocallyClosed n := by match A with
+  | .var _ =>
+    rw [Type_open] at Aoplc
+    split at Aoplc
+    · case isTrue h' =>
+      rw [← h']
+      exact var_bound h
+    · case isFalse h' => exact Aoplc
+  | .lam .. =>
+    rw [Type_open] at Aoplc
+    let .lam A'oplc := Aoplc
+    exact lam <| A'oplc.Type_open_drop <| Nat.add_lt_add_iff_right.mpr h
+  | .app A' B =>
+    rw [Type_open] at Aoplc
+    let .app A'oplc Boplc := Aoplc
+    exact app (A'oplc.Type_open_drop h) (Boplc.Type_open_drop h)
+  | .forall .. =>
+    rw [Type_open] at Aoplc
+    let .forall A'oplc := Aoplc
+    exact «forall» <| A'oplc.Type_open_drop <| Nat.add_lt_add_iff_right.mpr h
+  | .arr .. =>
+    rw [Type_open] at Aoplc
+    let .arr A'oplc Boplc := Aoplc
+    exact arr (A'oplc.Type_open_drop h) (Boplc.Type_open_drop h)
+  | .list A's =>
+    rw [Type_open] at Aoplc
+    match h' : A's with
+    | [] => exact .list fun _ => (nomatch ·)
+    | A' :: A's' =>
+      apply list
+      intro A'' A''in
+      let .list A'oplc := Aoplc
+      match A''in with
+      | .head _ => exact A'oplc (A''.Type_open _ _) (.head _) |>.Type_open_drop h
+      | .tail _ A''inA's' =>
+        have := list <| fun A''' A'''in => A'oplc A''' <| .tail _ A'''in
+        rw [← Type_open] at this
+        let .list A's'lc := this.Type_open_drop h
+        exact A's'lc A'' A''inA's'
+  | .listApp A' B =>
+    rw [Type_open] at Aoplc
+    let .listApp A'oplc Boplc := Aoplc
+    exact listApp (A'oplc.Type_open_drop h) (Boplc.Type_open_drop h)
+  | .prod A' =>
+    rw [Type_open] at Aoplc
+    let .prod A'oplc := Aoplc
+    exact prod <| A'oplc.Type_open_drop h
+  | .sum A' =>
+    rw [Type_open] at Aoplc
+    let .sum A'oplc := Aoplc
+    exact sum <| A'oplc.Type_open_drop h
+termination_by sizeOf A
+decreasing_by
+  all_goals simp_arith
+  · apply Nat.le_of_lt
+    apply List.sizeOf_lt_of_mem
+    have : A's = A' :: A's' := by assumption
+    cases this
+    exact A''in
+  · have : A's = A' :: A's' := by assumption
+    cases this
+    simp_arith
 
 theorem TypeVar_open_drop {A : «Type»} (h : m < n)
   (Aoplc : (A.TypeVar_open a m).TypeVarLocallyClosed n) : A.TypeVarLocallyClosed n := by
@@ -210,19 +294,94 @@ theorem TypeVar_open_eq {A : «Type»} (Alc : A.TypeVarLocallyClosed n) : A.Type
   | .prod .. => let .prod A'lc := Alc; rw [TypeVar_open, A'lc.TypeVar_open_eq]
   | .sum .. => let .sum A'lc := Alc; rw [TypeVar_open, A'lc.TypeVar_open_eq]
 
+theorem TypeVar_open_TypeVar_close_id
+  : TypeVarLocallyClosed A n → (A.TypeVar_close a n).TypeVar_open a n = A := by
+  induction A using rec_uniform generalizing n <;> aesop
+    (add simp [TypeVar_open, TypeVar_close], 40% cases TypeVarLocallyClosed,
+      safe List.map_eq_id_of_eq_id_of_mem)
+
+theorem Type_open_var_TypeVar_close_id
+  : TypeVarLocallyClosed A n → (A.TypeVar_close a n).Type_open (.var a) n = A := by
+  rw [← TypeVar_open_eq_Type_open_var]
+  exact TypeVar_open_TypeVar_close_id
+
+theorem Type_open_TypeVar_open_comm
+  : TypeVarLocallyClosed B n → m ≠ n →
+    (Type_open A B m).TypeVar_open a n = (A.TypeVar_open a n).Type_open B m := by
+  induction A using rec_uniform generalizing m n <;> aesop
+    (add simp [Type_open, TypeVar_open], 40% TypeVar_open_eq, safe weaken)
+
+theorem Type_open_TypeVar_open_eq
+  : TypeVarLocallyClosed B n → (Type_open A B n).TypeVar_open a n = A.Type_open B n := by
+  induction A using rec_uniform generalizing n <;> aesop
+    (add simp [Type_open, TypeVar_open], 40% TypeVar_open_eq, safe weaken)
+
+theorem Type_open_intro (Alc : A.TypeVarLocallyClosed n) (Blc : B.TypeVarLocallyClosed n)
+  : (Type_open A B m).TypeVarLocallyClosed n := by
+  induction Alc generalizing m <;> aesop
+    (add simp Type.Type_open, safe constructors TypeVarLocallyClosed, 40% weaken)
+
+theorem Type_open_dec (Alc : TypeVarLocallyClosed A (n + 1)) (Blc : B.TypeVarLocallyClosed n)
+  : (Type_open A B n).TypeVarLocallyClosed n := by
+  match A with
+  | .var (.bound _) =>
+    rw [Type_open]
+    split
+    · case _ => exact Blc
+    · case _ h =>
+      let .var_bound lt := Alc
+      exact var_bound <| Nat.lt_of_le_of_ne (Nat.le_of_lt_succ lt) <|
+        Ne.symm (h <| TypeVar.bound.injEq .. |>.mpr ·)
+  | .var (.free _) =>
+    rw [Type_open]
+    exact var_free
+  | .lam .. =>
+    rw [Type_open]
+    let .lam A'lc := Alc
+    exact lam <| A'lc.Type_open_dec Blc.weaken
+  | .app .. =>
+    rw [Type_open]
+    let .app A'lc B'lc := Alc
+    exact app (A'lc.Type_open_dec Blc) (B'lc.Type_open_dec Blc)
+  | .forall .. =>
+    rw [Type_open]
+    let .forall A'lc := Alc
+    exact «forall» <| A'lc.Type_open_dec Blc.weaken
+  | .arr .. =>
+    rw [Type_open]
+    let .arr A'lc B'lc := Alc
+    exact arr (A'lc.Type_open_dec Blc) (B'lc.Type_open_dec Blc)
+  | .list .. =>
+    let .list Aslc := Alc
+    rw [Type_open, List.mapMem_eq_map]
+    exact list fun A' mem => by
+      let ⟨A'', mem', eq⟩ := List.mem_map.mp mem
+      cases eq
+      exact Aslc A'' mem' |>.Type_open_dec Blc
+  | .listApp .. =>
+    rw [Type_open]
+    let .listApp A'lc B'lc := Alc
+    exact listApp (A'lc.Type_open_dec Blc) (B'lc.Type_open_dec Blc)
+  | .prod .. =>
+    rw [Type_open]
+    let .prod A'lc := Alc
+    exact prod <| A'lc.Type_open_dec Blc
+  | .sum .. =>
+    rw [Type_open]
+    let .sum A'lc := Alc
+    exact sum <| A'lc.Type_open_dec Blc
+
 end TypeVarLocallyClosed
 
-@[elab_as_elim]
-def rec_uniform {motive : «Type» → Prop} (var : ∀ a : TypeVar, motive (var a))
-  (lam : ∀ K A, motive A → motive (lam K A)) (app : ∀ A B, motive A → motive B → motive (app A B))
-  («forall» : ∀ K A, motive A → motive («forall» K A))
-  (arr : ∀ A B, motive A → motive B → motive (arr A B))
-  (list : ∀ As, (∀ A ∈ As, motive A) → motive (list As))
-  (listApp : ∀ A B, motive A → motive B → motive (listApp A B))
-  (prod : ∀ A, motive A → motive (prod A)) (sum : ∀ A, motive A → motive (sum A)) (A : «Type»)
-  : motive A :=
-  rec (motive_1 := motive) var lam app «forall» arr list listApp prod sum (fun _ => (nomatch ·))
-    (fun _ _ ih₀ ih₁ _ mem => match mem with | .head _ => ih₀ | .tail _ mem' => ih₁ _ mem') A
+theorem TypeVar_close_eq_of_not_mem_freeTypeVars
+  : a ∉ freeTypeVars A → A.TypeVar_close a n = A := by
+  induction A using rec_uniform generalizing n <;> aesop (add simp [freeTypeVars, TypeVar_close])
+
+theorem TypeVar_close_TypeVar_open_eq_of_not_mem_freeTypeVars
+  : a ∉ freeTypeVars A → (A.TypeVar_open a n).TypeVar_close a n = A := by
+  induction A using rec_uniform generalizing n <;> aesop
+    (add simp [freeTypeVars, TypeVar_open, TypeVar_close],
+      safe List.map_eq_id_of_eq_id_of_mem)
 
 theorem TypeVar_open_not_mem_freeTypeVars_preservation_of_ne
   : a ≠ a' → a ∉ freeTypeVars A → a ∉ (A.TypeVar_open a' n).freeTypeVars := by
@@ -234,8 +393,11 @@ theorem TypeVar_open_inj_of_not_mem_freeTypeVars (aninA : a ∉ freeTypeVars A)
   (aninB : a ∉ freeTypeVars B) (eq : A.TypeVar_open a n = B.TypeVar_open a n) : A = B := by
   induction A using rec_uniform generalizing B n <;>
     induction B using rec_uniform <;> aesop
-    (add simp [TypeVar_open, freeTypeVars], safe cases TypeVar,
-      10% apply List.eq_of_map_eq_map_of_inj)
+    (add simp [TypeVar_open, freeTypeVars], safe cases TypeVar, 10% List.eq_of_map_eq_map_of_inj)
+
+theorem not_mem_freeTypeVars_TypeVar_close : a ∉ (TypeVar_close A a n).freeTypeVars := by
+  induction A using rec_uniform generalizing n <;> aesop
+    (add simp [TypeVar_close, freeTypeVars], safe cases TypeVar)
 
 end «Type»
 
@@ -413,10 +575,10 @@ namespace TypeEquivalence
 private
 def symm : [[Δ ⊢ A ≡ B]] → [[Δ ⊢ B ≡ A]]
   | refl => refl
-  | lamAppL h => lamAppR h
-  | lamAppR h => lamAppL h
-  | lamListAppL h => lamListAppR h
-  | lamListAppR h => lamListAppL h
+  | lamAppL => lamAppR
+  | lamAppR => lamAppL
+  | listAppL => listAppR
+  | listAppR => listAppL
   | lam I h => lam I fun a mem => (h a mem).symm
   | app h₁ h₂ => app h₁.symm h₂.symm
   | scheme I h => scheme I fun a mem => (h a mem).symm
@@ -426,7 +588,6 @@ def symm : [[Δ ⊢ A ≡ B]] → [[Δ ⊢ B ≡ A]]
   | prod h => prod h.symm
   | sum h => sum h.symm
 
-private
 def trans : [[Δ ⊢ A₀ ≡ A₁]] → [[Δ ⊢ A₁ ≡ A₂]] → [[Δ ⊢ A₀ ≡ A₂]] := sorry
 
 end TypeEquivalence
