TabularTypeInterpreter/F⊗⊕ω/Lemmas/Environment.lean
@@ -1,0 +1,2 @@
+import TabularTypeInterpreter.«F⊗⊕ω».Lemmas.Environment.Basic
+import TabularTypeInterpreter.«F⊗⊕ω».Lemmas.Environment.EnvironmentWellFormedness
