TabularTypeInterpreter/F⊗⊕ω/Lemmas/Environment/Basic.lean
@@ -1,0 +1,12 @@
+import TabularTypeInterpreter.«F⊗⊕ω».Semantics.Environment
+
+namespace TabularTypeInterpreter.«F⊗⊕ω».Environment
+
+theorem append_empty (Δ : Environment) : Δ.append empty = Δ := rfl
+
+theorem empty_append (Δ : Environment) : append empty Δ = Δ := by
+  match Δ with
+  | empty => rfl
+  | typeExt Δ' .. | termExt Δ' .. => rw [append, Δ'.empty_append]
+
+end TabularTypeInterpreter.«F⊗⊕ω».Environment
