TabularTypeInterpreter/F⊗⊕ω/Lemmas/Environment/EnvironmentWellFormedness.lean
@@ -1,0 +1,23 @@
+import TabularTypeInterpreter.«F⊗⊕ω».Lemmas.Type
+import TabularTypeInterpreter.«F⊗⊕ω».Semantics.Environment
+
+theorem TabularTypeInterpreter.«F⊗⊕ω».EnvironmentWellFormedness.to_Kinding_of_TermVarIn
+  (Δwf : [[⊢ Δ]]) (xAinΔ : [[x : A ∈ Δ]]) : [[Δ ⊢ A : *]] := by match Δwf with
+  | .empty => nomatch xAinΔ
+  | .typeVarExt Δ'wf aninΔ' (Δ := Δ') =>
+    let .typeVarExt xAinΔ' := xAinΔ
+    rw [← Δ'.empty_append]
+    exact Δ'wf.to_Kinding_of_TermVarIn xAinΔ' |>.weakening (Δ'' := .typeExt .empty ..) <| by
+      rw [Environment.empty_append]
+      exact Δ'wf.typeVarExt aninΔ'
+  | .termVarExt Δ'wf x'ninΔ' A'ki (Δ := Δ') => match xAinΔ with
+    | .head =>
+      rw [← Δ'.empty_append]
+      exact A'ki.weakening (Δ'' := .termExt .empty ..) <| by
+        rw [Environment.empty_append]
+        exact Δ'wf.termVarExt x'ninΔ' A'ki
+    | .termVarExt xAinΔ' _ =>
+      rw [← Δ'.empty_append]
+      exact Δ'wf.to_Kinding_of_TermVarIn xAinΔ' |>.weakening (Δ'' := .termExt .empty ..) <| by
+        rw [Environment.empty_append]
+        exact Δ'wf.termVarExt x'ninΔ' A'ki
