TabularTypeInterpreter/Lemmas/TypeEnvironment.lean
@@ -1,7 +1,15 @@
+import Aesop
 import TabularTypeInterpreter.Semantics.Type.KindingAndElaboration
 import TabularTypeInterpreter.Theorems.Kind
 
 namespace TabularTypeInterpreter.TypeEnvironment
+
+theorem append_empty (Γ : TypeEnvironment) : Γ.append empty = Γ := rfl
+
+theorem empty_append (Γ : TypeEnvironment) : append empty Γ = Γ := by
+  match Γ with
+  | empty => rfl
+  | typeExt Γ' .. | termExt Γ' .. | constrExt Γ' .. => rw [append, Γ'.empty_append]
 
 namespace WellFormednessAndElaboration
 
@@ -30,9 +38,67 @@ theorem TermVarNotInDom_preservation (Γwe : [[Γc ⊢ Γ ⇝ Δ]]) (xnin : [[x 
     | .inl (.refl _) => xnin <| .head _
     | .inr xinΔ' => Γ'we.TermVarNotInDom_preservation (List.not_mem_of_not_mem_cons xnin) xinΔ'
 
+theorem append_left_elim (ΓΓ'we : [[Γc ⊢ Γ, Γ' ⇝ Δ]]) : ∃ Δ', [[Γc ⊢ Γ ⇝ Δ']] := match Γ' with
+  | .empty => ⟨_, ΓΓ'we⟩
+  | .termExt .. => let .termExt ΓΓ''we .. := ΓΓ'we; ΓΓ''we.append_left_elim
+  | .typeExt .. => let .typeExt ΓΓ''we .. := ΓΓ'we; ΓΓ''we.append_left_elim
+  | .constrExt .. => let .constrExt ΓΓ''we .. := ΓΓ'we; ΓΓ''we.append_left_elim
+
 end WellFormednessAndElaboration
 
-theorem TypeVarIn.deterministic (aκ₀in : [[a : κ₀ ∈ Γ]]) (aκ₁in : [[a : κ₁ ∈ Γ]])
+namespace TypeVarIn
+
+theorem append_elim (aκin : [[a : κ ∈ Γ, Γ']])
+  : ([[a : κ ∈ Γ]] ∧ [[a ∉ dom(Γ')]]) ∨ [[a : κ ∈ Γ']] := match Γ' with
+  | .empty => .inl ⟨aκin, (nomatch ·)⟩
+  | .typeExt .. => match aκin with
+    | head => .inr head
+    | typeExt ne aκin' => match aκin'.append_elim with
+      | .inl ⟨aκinΓ, aκninΓ''⟩ =>
+        .inl <| ⟨aκinΓ, fun | .head _ => nomatch ne | .tail _ mem => aκninΓ'' mem⟩
+      | .inr aκinΓ'' => .inr <| aκinΓ''.typeExt ne
+  | .termExt .. => let .termExt aκin' .. := aκin; aκin'.append_elim.imp_right termExt
+  | .constrExt .. => let .constrExt aκin' .. := aκin; aκin'.append_elim.imp_right constrExt
+
+theorem append_inl (aκin : [[a : κ ∈ Γ]]) (anin : [[a ∉ dom(Γ')]]) : [[a : κ ∈ Γ, Γ']] := by
+  match Γ' with
+  | .empty => exact aκin
+  | .typeExt .. =>
+    let ⟨ne, anin'⟩ := List.not_mem_cons.mp anin
+    exact aκin.append_inl anin' |>.typeExt ne
+  | .termExt .. =>
+    rw [TypeVarNotInDom, typeVarDom] at anin
+    exact aκin.append_inl anin |>.termExt
+  | .constrExt .. =>
+    rw [TypeVarNotInDom, typeVarDom] at anin
+    exact aκin.append_inl anin |>.constrExt
+
+theorem append_inr : [[a : κ ∈ Γ]] → [[a : κ ∈ Γ', Γ]]
+  | head => .head
+  | typeExt ne aκin' => aκin'.append_inr.typeExt ne
+  | termExt aκin' => aκin'.append_inr.termExt
+  | constrExt aκin' => aκin'.append_inr.constrExt
+
+theorem not_of_NotInDom (anin : [[a ∉ dom(Γ)]]) (aκin : [[a : κ ∈ Γ]]) : False := by match Γ with
+  | .empty => nomatch aκin
+  | .typeExt .. => match aκin with
+    | .head => nomatch List.ne_of_not_mem_cons anin
+    | .typeExt ne aκin' => exact aκin'.not_of_NotInDom <| List.not_mem_of_not_mem_cons anin
+  | .termExt .. =>
+    let .termExt aκin' := aκin
+    rw [TypeVarNotInDom, typeVarDom] at anin
+    exact aκin'.not_of_NotInDom anin
+  | .constrExt .. =>
+    let .constrExt aκin' := aκin
+    rw [TypeVarNotInDom, typeVarDom] at anin
+    exact aκin'.not_of_NotInDom anin
+
+theorem append_elim_left (aκin : [[a : κ ∈ Γ, Γ']]) (anin : [[a ∉ dom(Γ')]]) : [[a : κ ∈ Γ]] :=
+  match aκin.append_elim with
+  | .inl ⟨aκinΓ, _⟩ => aκinΓ
+  | .inr aκinΓ' => nomatch aκinΓ'.not_of_NotInDom anin
+
+theorem deterministic (aκ₀in : [[a : κ₀ ∈ Γ]]) (aκ₁in : [[a : κ₁ ∈ Γ]])
   : κ₀ = κ₁ := match Γ with
   | .empty => nomatch aκ₀in
   | .typeExt .. => by
@@ -53,5 +119,16 @@ theorem TypeVarIn.deterministic (aκ₀in : [[a : κ₀ ∈ Γ]]) (aκ₁in : [[
     let .constrExt aκ₀in' := aκ₀in
     let .constrExt aκ₁in' := aκ₁in
     aκ₀in'.deterministic aκ₁in'
+
+theorem TypeVar_subst_preservation : [[a : κ ∈ Γ]] → [[a : κ ∈ Γ [τ / a'] ]]
+  | .head => .head
+  | .typeExt ne aκin' => aκin'.TypeVar_subst_preservation.typeExt ne
+  | .termExt aκin' => aκin'.TypeVar_subst_preservation.termExt
+  | .constrExt aκin' => aκin'.TypeVar_subst_preservation.constrExt
+
+end TypeVarIn
+
+theorem TypeVarNotInDom.TypeVar_subst_preservation :[[a ∉ dom(Γ)]] → [[a ∉ dom(Γ [τ / a'])]] := by
+  induction Γ <;> aesop (add simp [TypeVarNotInDom, typeVarDom])
 
 end TabularTypeInterpreter.TypeEnvironment
