TabularTypeInterpreter/Theorems/Type/Basic.lean
@@ -1,0 +1,410 @@
+import TabularTypeInterpreter.«F⊗⊕ω».Lemmas.Term
+import TabularTypeInterpreter.«F⊗⊕ω».Lemmas.Type
+import TabularTypeInterpreter.«F⊗⊕ω».Semantics.Environment
+import TabularTypeInterpreter.Lemmas.ClassEnvironment
+import TabularTypeInterpreter.Lemmas.Type
+import TabularTypeInterpreter.Lemmas.TypeEnvironment
+import TabularTypeInterpreter.Semantics.Type
+import TabularTypeInterpreter.Theorems.Kind
+
+namespace TabularTypeInterpreter
+
+open «F⊗⊕ω»
+open Std
+
+theorem Monotype.RowEquivalenceAndElaboration.soundness (ρee : [[Γc; Γ ⊢ ρ₀ ≡(μ) ρ₁ ⇝ Fₚ, Fₛ]])
+  (Γwe : [[Γc ⊢ Γ ⇝ Δ]]) (ρ₀ke : [[Γc; Γ ⊢ ρ₀ : R κ ⇝ A]]) (ρ₁ke : [[Γc; Γ ⊢ ρ₁ : R κ ⇝ B]])
+  (κe : [[⊢ κ ⇝ K]])
+  : [[Δ ⊢ Fₚ : ∀ a : K ↦ *. (⊗ (a$0 ⟦A⟧)) → ⊗ (a$0 ⟦B⟧)]] ∧
+    [[Δ ⊢ Fₛ : ∀ a : K ↦ *. (⊕ (a$0 ⟦A⟧)) → ⊕ (a$0 ⟦B⟧)]] ∧
+    Fₚ.TypeVarLocallyClosed ∧ Fₛ.TypeVarLocallyClosed := by match ρee with
+  | refl ρ₀ke' κe' =>
+    let ⟨κeq, Aeq⟩ := ρ₀ke.deterministic ρ₀ke'
+    cases κeq
+    cases Aeq
+    cases κe.deterministic κe'
+    cases ρ₀ke.deterministic ρ₁ke |>.right
+    let Δwf := Γwe.soundness
+    let Aki := ρ₀ke.soundness Γwe κe.row
+    let Alc := Aki.TypeVarLocallyClosed_of
+    exact ⟨.prod_id Δwf Aki, .sum_id Δwf Aki, .prod_id Alc, .sum_id Alc⟩
+  | trans ρ₀ke' κe' ρ₀₁ee ρ₁₂ee =>
+    let ⟨κeq, Aeq⟩ := ρ₀ke.deterministic ρ₀ke'
+    cases κeq
+    cases Aeq
+    cases κe.deterministic κe'
+    let ⟨_, _, A₁, ρ₀ke'', ρ₁ke'⟩ := ρ₀₁ee.to_Kinding Γwe
+    cases ρ₀ke'.deterministic ρ₀ke'' |>.left
+    let ⟨Fₚ₀₁ty, Fₛ₀₁ty, Fₚ₀₁lc, Fₛ₀₁lc⟩ := ρ₀₁ee.soundness Γwe ρ₀ke ρ₁ke' κe
+    let ⟨_, _, A₂, ρ₁ke'', ρ₂ke⟩ := ρ₁₂ee.to_Kinding Γwe
+    cases ρ₁ke'.deterministic ρ₁ke'' |>.left
+    cases ρ₁ke.deterministic ρ₂ke |>.right
+    let ⟨Fₚ₁₂ty, Fₛ₁₂ty, Fₚ₁₂lc, Fₛ₁₂lc⟩ := ρ₁₂ee.soundness Γwe ρ₁ke' ρ₂ke κe
+    let Δwf := Γwe.soundness
+    let I := A.freeTypeVars ++ A₁.freeTypeVars ++ B.freeTypeVars ++ Δ.typeVarDom
+    let Aki := ρ₀ke.soundness Γwe κe.row
+    let Alc := Aki.TypeVarLocallyClosed_of
+    let A₁lc := ρ₁ke'.soundness Γwe κe.row |>.TypeVarLocallyClosed_of
+    let Blc := ρ₁ke.soundness Γwe κe.row |>.TypeVarLocallyClosed_of
+    exact ⟨
+      .typeLam (I := I) fun a anin => by
+        let ⟨aninAA₁B, aninΔ⟩ := List.not_mem_append'.mp anin
+        let ⟨aninAA₁, aninB⟩ := List.not_mem_append'.mp aninAA₁B
+        let ⟨aninA, aninA₁⟩ := List.not_mem_append'.mp aninAA₁
+        let Δa := Δ.typeExt a (K.arr .star)
+        let Δawf : [[⊢ Δa]] := Δwf.typeVarExt aninΔ
+        simp only [«F⊗⊕ω».Term.TypeVar_open, Type.TypeVar_open, if_pos]
+        exact .lam (I := Δ.termVarDom) fun x xnin => by
+          simp only [«F⊗⊕ω».Term.TermVar_open, if_pos]
+          rw [Fₚ₀₁lc.TypeVar_open_eq, Fₚ₁₂lc.TypeVar_open_eq,
+              Fₚ₀₁ty.TermVarLocallyClosed_of.TermVar_open_eq,
+              Fₚ₁₂ty.TermVarLocallyClosed_of.TermVar_open_eq]
+          rw [Alc.TypeVar_open_eq]
+          let Δax := Δa.termExt x [[⊗ (a ⟦A⟧)]]
+          let Δaxwf := Δawf.termVarExt xnin <| by
+            rw [← Δa.empty_append] at Δawf ⊢
+            exact .prod <| .listApp (.var .head) <| Aki.weakening Δawf (Δ'' := .typeExt .empty ..)
+          apply Typing.app (A := [[⊗ (a ⟦A₁⟧)]])
+          · rw [← Type.TypeVarLocallyClosed.Type_open_var_TypeVar_close_id (A := .arr ..) <| by
+                  rw [Blc.TypeVar_open_eq]
+                  exact .arr (.prod (.listApp .var_free A₁lc)) (.prod (.listApp .var_free Blc))]
+            apply Typing.typeApp _ <| .var <| .termVarExt .head
+            rw [← (Δa.termExt x ..).empty_append]
+            simp only [Type.TypeVar_close, if_pos]
+            rw [Type.TypeVar_close_eq_of_not_mem_freeTypeVars aninA₁,
+                Type.TypeVar_close_TypeVar_open_eq_of_not_mem_freeTypeVars aninB]
+            apply Fₚ₁₂ty.weakening _ (Δ'' := .termExt (.typeExt .empty ..) ..)
+            rw [Environment.empty_append]
+            exact Δaxwf
+          · apply Typing.app (A := [[⊗ (a ⟦A⟧)]])
+            · rw [← Type.TypeVarLocallyClosed.Type_open_var_TypeVar_close_id <|
+                    .arr (.prod (.listApp .var_free Alc)) (.prod (.listApp .var_free A₁lc))]
+              apply Typing.typeApp _ <| .var <| .termVarExt .head
+              rw [← ((Δ.typeExt ..).termExt ..).empty_append]
+              simp only [Type.TypeVar_close, if_pos]
+              rw [Type.TypeVar_close_eq_of_not_mem_freeTypeVars aninA,
+                  Type.TypeVar_close_eq_of_not_mem_freeTypeVars aninA₁]
+              apply Fₚ₀₁ty.weakening _ (Δ'' := .termExt (.typeExt .empty ..) ..)
+              rw [Environment.empty_append]
+              exact Δaxwf
+            · exact .var Δaxwf .head,
+      .typeLam (I := I) fun a anin => by
+        let ⟨aninAA₁B, aninΔ⟩ := List.not_mem_append'.mp anin
+        let ⟨aninAA₁, aninB⟩ := List.not_mem_append'.mp aninAA₁B
+        let ⟨aninA, aninA₁⟩ := List.not_mem_append'.mp aninAA₁
+        let Δa := Δ.typeExt a (K.arr .star)
+        let Δawf : [[⊢ Δa]] := Δwf.typeVarExt aninΔ
+        simp only [«F⊗⊕ω».Term.TypeVar_open, Type.TypeVar_open, if_pos]
+        exact .lam (I := Δ.termVarDom) fun x xnin => by
+          simp only [«F⊗⊕ω».Term.TermVar_open, if_pos]
+          rw [Fₛ₀₁lc.TypeVar_open_eq, Fₛ₁₂lc.TypeVar_open_eq,
+              Fₛ₀₁ty.TermVarLocallyClosed_of.TermVar_open_eq,
+              Fₛ₁₂ty.TermVarLocallyClosed_of.TermVar_open_eq]
+          rw [Alc.TypeVar_open_eq]
+          let Δax := Δa.termExt x [[⊕ (a ⟦A⟧)]]
+          let Δaxwf := Δawf.termVarExt xnin <| by
+            rw [← Δa.empty_append] at Δawf ⊢
+            exact .sum <| .listApp (.var .head) <| Aki.weakening Δawf (Δ'' := .typeExt .empty ..)
+          apply Typing.app (A := [[⊕ (a ⟦A₁⟧)]])
+          · rw [← Type.TypeVarLocallyClosed.Type_open_var_TypeVar_close_id (A := .arr ..) <| by
+                  rw [Blc.TypeVar_open_eq]
+                  exact .arr (.sum (.listApp .var_free A₁lc)) (.sum (.listApp .var_free Blc))]
+            apply Typing.typeApp _ <| .var <| .termVarExt .head
+            simp only [Type.TypeVar_close, if_pos]
+            rw [Type.TypeVar_close_eq_of_not_mem_freeTypeVars aninA₁,
+                Type.TypeVar_close_TypeVar_open_eq_of_not_mem_freeTypeVars aninB]
+            rw [← (Δa.termExt x ..).empty_append] at Δaxwf ⊢
+            exact Fₛ₁₂ty.weakening Δaxwf (Δ'' := .termExt (.typeExt .empty ..) ..)
+          · apply Typing.app (A := [[⊕ (a ⟦A⟧)]])
+            · rw [← Type.TypeVarLocallyClosed.Type_open_var_TypeVar_close_id <|
+                    .arr (.sum (.listApp .var_free Alc)) (.sum (.listApp .var_free A₁lc))]
+              apply Typing.typeApp _ <| .var <| .termVarExt .head
+              simp only [Type.TypeVar_close, if_pos]
+              rw [Type.TypeVar_close_eq_of_not_mem_freeTypeVars aninA,
+                  Type.TypeVar_close_eq_of_not_mem_freeTypeVars aninA₁]
+              rw [← ((Δ.typeExt ..).termExt ..).empty_append] at Δaxwf ⊢
+              exact Fₛ₀₁ty.weakening Δaxwf (Δ'' := .termExt (.typeExt .empty ..) ..)
+            · exact .var Δaxwf .head,
+      .typeLam <| .lam (.prod <| .listApp (.var_bound Nat.one_pos) Alc.weaken) <|
+        .app (.typeApp Fₚ₁₂lc.weaken (.var_bound Nat.one_pos)) <|
+        .app (.typeApp Fₚ₀₁lc.weaken (.var_bound Nat.one_pos)) .var,
+      .typeLam <| .lam (.sum <| .listApp (.var_bound Nat.one_pos) Alc.weaken) <|
+        .app (.typeApp Fₛ₁₂lc.weaken (.var_bound Nat.one_pos)) <|
+        .app (.typeApp Fₛ₀₁lc.weaken (.var_bound Nat.one_pos)) .var
+    ⟩
+  | comm perm perm' inv ξτske κe' (A := A') (p := p) (p' := p') =>
+    rw [← Range.map_get!_eq (as := p)] at ρ₁ke ⊢
+    rw [List.map_map, ← Range.map] at ρ₁ke
+    let ⟨⟨_, ξke⟩, _, ⟨B', _, Beq, κeq, _, _, τke⟩⟩ := ρ₁ke.row_inversion
+    cases Beq
+    cases κeq
+    let ⟨κeq, Aeq⟩ := ξτske.deterministic ρ₀ke
+    cases κeq
+    cases Aeq
+    cases κe.deterministic κe'
+    let ⟨⟨_, _⟩, _, ⟨A'', _, eq, eqκ, _, _, τke'⟩⟩ := ρ₀ke.row_inversion
+    cases eqκ
+    rw [List.map_singleton_flatten, List.map_singleton_flatten] at eq
+    let A'eq := Range.eq_of_mem_of_map_eq <| Type.list.inj eq
+    let length_eq := perm.length_eq
+    rw [Range.length_toList] at length_eq
+    let length_eq' := perm'.length_eq
+    rw [Range.length_toList, Nat.sub_zero] at length_eq'
+    cases length_eq
+    let A'slc' := by
+      show ∀ i ∈ [:p.length], (A' i).TypeVarLocallyClosed 1
+      intro i mem
+      rw [A'eq i mem]
+      rw [← Nat.zero_add 1]
+      exact τke' i mem |>.soundness Γwe κe |>.TypeVarLocallyClosed_of.weaken
+    let A'slc := by
+      show ∀ A ∈ ([:p.length].map fun i => [A' i]).flatten, A.TypeVarLocallyClosed 1
+      intro A' mem
+      rw [List.map_singleton_flatten] at mem
+      let ⟨i, mem', eq⟩ := Std.Range.mem_of_mem_map mem
+      cases eq
+      exact A'slc' i mem'
+    exact ⟨
+      .typeLam (I := Δ.typeVarDom) fun a anin => by
+        simp only [«F⊗⊕ω».Term.TypeVar_open, Type.TypeVar_open, if_pos]
+        let Δawf := Γwe.soundness.typeVarExt anin (K := K.arr .star)
+        exact .lam (I := Δ.termVarDom) fun x xnin => by
+          simp only [«F⊗⊕ω».Term.TermVar_open, List.mapMem_eq_map, if_pos]
+          rw [List.map_singleton_flatten, List.map_singleton_flatten, List.map_singleton_flatten,
+              List.map_map, List.map_map, List.map_map, List.map_map, List.map_map,
+              ← List.map_singleton_flatten, ← Range.map, ← List.map_singleton_flatten,
+              ← Range.map, ← List.map_singleton_flatten, ← Range.map]
+          apply Typing.equiv _ <| .prod .listAppR
+          simp only [Function.comp, «F⊗⊕ω».Term.TypeVar_open, «F⊗⊕ω».Term.TermVar_open, if_pos]
+          apply Typing.prodIntro
+          intro i imem
+          simp only
+          rw [← inv.left i imem]
+          show Typing _ _
+            ((fun i => .app (.var (.free a)) ((B' (p'.get! i)).TypeVar_open a)) (p.get! i))
+          rw [inv.left i imem]
+          apply Typing.prodElim _
+            (Range.mem_of_mem_toList <| perm.mem_iff.mp <| List.get!_mem imem.right)
+            (A := fun i => .app (.var (.free a)) ((B' (p'.get! i)).TypeVar_open a))
+          apply Typing.equiv _ <| .prod .listAppL
+          rw [Range.map, Range.map_eq_of_eq_of_mem fun i imem => by
+                show [(A' i).TypeVar_open a] = [(B' (p'.get! i)).TypeVar_open a]
+                let iltlen := imem.right
+                rw [← length_eq'] at iltlen
+                let τeki := τke (p'.get! i) <| Range.mem_of_mem_toList <| perm'.mem_iff.mp <|
+                  List.get!_mem iltlen
+                let τek'i := τke' i imem
+                rw [← A'eq i imem] at τek'i
+                rw [inv.right i imem] at τeki
+                rw [τeki.deterministic τek'i |>.right] ]
+          apply Typing.var _ .head
+          apply Δawf |>.termVarExt xnin
+          apply Kinding.prod
+          apply Kinding.listApp <| .var .head
+          apply Kinding.list
+          intro i imem
+          let iltlen := imem.right
+          rw [← length_eq'] at iltlen
+          let τkei := τke (p'.get! i) <| Range.mem_of_mem_toList <| perm'.mem_iff.mp <|
+            List.get!_mem iltlen
+          let B'ki := τkei.soundness Γwe κe
+          simp only
+          rw [B'ki.TypeVarLocallyClosed_of.TypeVar_open_eq]
+          rw [← (Δ.typeExt ..).empty_append] at Δawf ⊢
+          exact B'ki.weakening Δawf (Δ'' := .typeExt .empty ..),
+      .typeLam (I := Δ.typeVarDom) fun a anin => by
+        simp only [«F⊗⊕ω».Term.TypeVar_open, Type.TypeVar_open, if_pos]
+        let Δa := Δ.typeExt a <| K.arr .star
+        let Δawf : [[⊢ Δa]] := Γwe.soundness.typeVarExt anin (K := K.arr .star)
+        exact .lam (I := Δ.termVarDom) fun x xnin => by
+          let Δaxwf := Δawf.termVarExt xnin <| by
+            apply Kinding.sum
+            apply Kinding.listApp <| .var .head
+            apply Kinding.list
+            intro i imem
+            show Kinding _ ((A' i).TypeVar_open a) _
+            let A'ki := τke' i imem |>.soundness Γwe κe
+            rw [← A'eq i imem] at A'ki
+            rw [← (Δ.typeExt ..).empty_append, A'ki.TypeVarLocallyClosed_of.TypeVar_open_eq]
+            apply A'ki.weakening (Δ'' := .typeExt .empty ..)
+            rw [Environment.empty_append]
+            exact Δawf
+          simp only [«F⊗⊕ω».Term.TermVar_open, List.mapMem_eq_map, if_pos]
+          rw [← Range.map_get!_eq (as := p'), length_eq', Range.map, List.map_singleton_flatten,
+              List.map_singleton_flatten, List.map_singleton_flatten, List.zip_eq_zipWith,
+              Range.map, List.zipWith_map_right, List.zipWith_same, List.map_map, List.map_map,
+              List.map_map, List.map_map, List.map_map, ← List.map_singleton_flatten,
+              ← Range.map, ← List.map_singleton_flatten, ← Range.map, ← List.map_singleton_flatten,
+              ← Range.map]
+          simp only [Function.comp]
+          apply Typing.sumElim
+          · exact .equiv (.var Δaxwf .head) <| .sum <| .listAppL
+          · intro i imem
+            simp only
+            simp only [Type.TypeVar_open, «F⊗⊕ω».Term.TypeVar_open, «F⊗⊕ω».Term.TermVar_open,
+                       if_pos]
+            rw [if_neg (nomatch ·)]
+            exact .lam (I := x :: Δa.termVarDom) fun x' x'nin => by
+              simp only [«F⊗⊕ω».Term.TermVar_open, if_pos]
+              apply Typing.equiv _ <| .sum <| .listAppR
+              let iltplen := imem.right
+              rw [← length_eq'] at iltplen
+              apply Typing.sumIntro <| Range.mem_of_mem_toList <| perm'.mem_iff.mp <|
+                List.get!_mem iltplen
+              let iltlen := imem.right
+              rw [← length_eq'] at iltlen
+              let τeki := τke (p'.get! i) <| Range.mem_of_mem_toList <| perm'.mem_iff.mp <|
+                List.get!_mem iltlen
+              let τek'i := τke' i imem
+              rw [← A'eq i imem] at τek'i
+              rw [inv.right i imem] at τeki
+              rw [← τeki.deterministic τek'i |>.right]
+              apply Typing.var _ .head
+              apply Δaxwf.termVarExt x'nin
+              apply Kinding.app
+              · exact .var <| .termVarExt <| .head
+              · let B'ki := τeki.soundness Γwe κe
+                rw [B'ki.TypeVarLocallyClosed_of.TypeVar_open_eq]
+                rw [← (Δa.termExt ..).empty_append] at Δaxwf ⊢
+                exact B'ki.weakening Δaxwf (Δ'' := .termExt (.typeExt .empty ..)  ..),
+      .typeLam <| .lam (.prod <| .listApp (.var_bound Nat.one_pos) (.list A'slc)) <|
+        .prodIntro fun E mem => by
+          rw [List.map_singleton_flatten, Range.map, List.map_map] at mem
+          let ⟨i, mem', eq⟩ := Std.Range.mem_of_mem_map mem
+          cases eq
+          simp only [Function.comp]
+          exact .prodElim .var,
+      .typeLam <| .lam (.sum <| .listApp (.var_bound Nat.one_pos) (.list A'slc)) <|
+        .sumElim .var fun E mem => by
+          rw [List.map_singleton_flatten, ← Range.map_get!_eq (as := p'), length_eq',
+              List.zip_eq_zipWith, Range.map, List.zipWith_map_right, List.zipWith_same,
+              List.map_map] at mem
+          let ⟨i, mem', eq⟩ := Std.Range.mem_of_mem_map mem
+          cases eq
+          simp only [Function.comp]
+          exact .lam (.app (.var_bound Nat.one_pos) <| A'slc' i mem') <| .sumIntro .var
+    ⟩
+  | liftL μ liftke@(.lift I τ₁ke κ₀e ξτ₀ke) κe' (τ₀ := τ₀) (τ₁ := τ₁) =>
+    rename_i A' _ _
+    let ⟨κeq, Aeq⟩ := liftke.deterministic ρ₀ke
+    cases κeq
+    cases Aeq
+    cases κe.deterministic κe'
+    let ⟨⟨_, ξke⟩, uni, ⟨A'', _, eq₀, eq₁, h, _, τ₀ke⟩⟩ := ξτ₀ke.row_inversion
+    cases eq₀
+    cases eq₁
+    let ξτopke := TypeScheme.KindingAndElaboration.row ξke uni (fun i imem =>
+      let σ := TypeScheme.qual (QualifiedType.mono τ₁)
+      let ⟨a, anin⟩ := σ.freeTypeVars ++ ↑A'.freeTypeVars ++ Γ.typeVarDom ++ I |>.exists_fresh
+      let ⟨aninσA'Γ, aninI⟩ := List.not_mem_append'.mp anin
+      let ⟨aninσA', aninΓ⟩ := List.not_mem_append'.mp aninσA'Γ
+      let ⟨aninσ, aninA'⟩ := List.not_mem_append'.mp aninσA'
+      τ₁ke a aninI |>.Monotype_open_preservation (Γ' := .empty) (Γwe.typeExt aninΓ κ₀e) (nomatch ·)
+        aninσ aninA' <| τ₀ke i imem) h
+    let ⟨κeq, Aeq⟩ := ξτopke.deterministic ρ₁ke
+    cases κeq
+    cases Aeq
+    let Δwf := Γwe.soundness
+    let Aki := ρ₀ke.soundness Γwe κe.row
+    let Alc := Aki.TypeVarLocallyClosed_of
+    exact ⟨
+      .equiv (.prod_id Δwf Aki) <| .scheme (I := []) fun a anin => by
+        simp only [Type.TypeVar_open, if_pos]
+        rw [List.mapMem_eq_map, List.mapMem_eq_map, Range.map, List.map_singleton_flatten,
+            List.map_singleton_flatten, List.map_map, List.map_map, ← List.map_singleton_flatten,
+            ← Range.map, ← List.map_singleton_flatten, ← Range.map]
+        simp only [Function.comp]
+        apply TypeEquivalence.arr .refl <| .prod <| .trans _ .listAppR
+        apply TypeEquivalence.trans (.listApp .refl .listAppL) <| .trans .listAppL <| .list _
+        intro i imem
+        apply TypeEquivalence.app .refl <| .trans .lamAppL _
+        let .list A'opslc := ρ₁ke.soundness Γwe κe.row |>.TypeVarLocallyClosed_of
+        rw [List.map_singleton_flatten] at A'opslc
+        let A''ilc := τ₀ke i imem |>.soundness Γwe κ₀e |>.TypeVarLocallyClosed_of
+        rw [A''ilc.TypeVar_open_eq, A'opslc (A'.Type_open (A'' i)) (Range.mem_map_of_mem imem)
+              |>.weaken (n := 1) |>.Type_open_drop (n := 1) Nat.one_pos |>.TypeVar_open_eq,
+            A''ilc.Type_open_TypeVar_open_eq]
+        exact .refl,
+     .equiv (.sum_id Δwf Aki) <| .scheme (I := []) fun a anin => by
+        simp only [Type.TypeVar_open, if_pos]
+        rw [List.mapMem_eq_map, List.mapMem_eq_map, Range.map, List.map_singleton_flatten,
+            List.map_singleton_flatten, List.map_map, List.map_map, ← List.map_singleton_flatten,
+            ← Range.map, ← List.map_singleton_flatten, ← Range.map]
+        simp only [Function.comp]
+        apply TypeEquivalence.arr .refl <| .sum <| .trans _ .listAppR
+        apply TypeEquivalence.trans (.listApp .refl .listAppL) <| .trans .listAppL <| .list _
+        intro i imem
+        apply TypeEquivalence.app .refl <| .trans .lamAppL _
+        let .list A'opslc := ρ₁ke.soundness Γwe κe.row |>.TypeVarLocallyClosed_of
+        rw [List.map_singleton_flatten] at A'opslc
+        let A''ilc := τ₀ke i imem |>.soundness Γwe κ₀e |>.TypeVarLocallyClosed_of
+        rw [A''ilc.TypeVar_open_eq, A'opslc (A'.Type_open (A'' i)) (Range.mem_map_of_mem imem)
+              |>.weaken (n := 1) |>.Type_open_drop (n := 1) Nat.one_pos |>.TypeVar_open_eq,
+            A''ilc.Type_open_TypeVar_open_eq]
+        exact .refl,
+      .prod_id Alc,
+      .sum_id Alc
+    ⟩
+  | liftR μ liftke@(.lift I τ₁ke κ₀e ξτ₀ke) κe' (τ₀ := τ₀) (τ₁ := τ₁) =>
+    rename_i A' _ _
+    let ⟨κeq, Aeq⟩ := liftke.deterministic ρ₁ke
+    cases κeq
+    cases Aeq
+    cases κe.deterministic κe'
+    let ⟨⟨_, ξke⟩, uni, ⟨A'', _, eq₀, eq₁, h, _, τ₀ke⟩⟩ := ξτ₀ke.row_inversion
+    cases eq₀
+    cases eq₁
+    let ξτopke := TypeScheme.KindingAndElaboration.row ξke uni (fun i imem =>
+      let σ := TypeScheme.qual (QualifiedType.mono τ₁)
+      let ⟨a, anin⟩ := σ.freeTypeVars ++ ↑A'.freeTypeVars ++ Γ.typeVarDom ++ I |>.exists_fresh
+      let ⟨aninσA'Γ, aninI⟩ := List.not_mem_append'.mp anin
+      let ⟨aninσA', aninΓ⟩ := List.not_mem_append'.mp aninσA'Γ
+      let ⟨aninσ, aninA'⟩ := List.not_mem_append'.mp aninσA'
+      τ₁ke a aninI |>.Monotype_open_preservation (Γ' := .empty) (Γwe.typeExt aninΓ κ₀e) (nomatch ·)
+        aninσ aninA' <| τ₀ke i imem) h
+    let ⟨κeq, Aeq⟩ := ξτopke.deterministic ρ₀ke
+    cases κeq
+    cases Aeq
+    let Δwf := Γwe.soundness
+    let Aki := ρ₁ke.soundness Γwe κe.row
+    let Alc := Aki.TypeVarLocallyClosed_of
+    exact ⟨
+      .equiv (.prod_id Δwf Aki) <| .scheme (I := []) fun a anin => by
+        simp only [Type.TypeVar_open, if_pos]
+        rw [List.mapMem_eq_map, List.mapMem_eq_map, Range.map, List.map_singleton_flatten,
+            List.map_singleton_flatten, List.map_map, List.map_map, ← List.map_singleton_flatten,
+            ← Range.map, ← List.map_singleton_flatten, ← Range.map]
+        simp only [Function.comp]
+        apply TypeEquivalence.arr (.prod <| .trans _ .listAppR) .refl
+        apply TypeEquivalence.trans (.listApp .refl .listAppL) <| .trans .listAppL <| .list _
+        intro i imem
+        apply TypeEquivalence.app .refl <| .trans .lamAppL _
+        let .list A'opslc := ρ₀ke.soundness Γwe κe.row |>.TypeVarLocallyClosed_of
+        rw [List.map_singleton_flatten] at A'opslc
+        let A''ilc := τ₀ke i imem |>.soundness Γwe κ₀e |>.TypeVarLocallyClosed_of
+        rw [A''ilc.TypeVar_open_eq, A'opslc (A'.Type_open (A'' i)) (Range.mem_map_of_mem imem)
+              |>.weaken (n := 1) |>.Type_open_drop (n := 1) Nat.one_pos |>.TypeVar_open_eq,
+            A''ilc.Type_open_TypeVar_open_eq]
+        exact .refl,
+      .equiv (.sum_id Δwf Aki) <| .scheme (I := []) fun a anin => by
+        simp only [Type.TypeVar_open, if_pos]
+        rw [List.mapMem_eq_map, List.mapMem_eq_map, Range.map, List.map_singleton_flatten,
+            List.map_singleton_flatten, List.map_map, List.map_map, ← List.map_singleton_flatten,
+            ← Range.map, ← List.map_singleton_flatten, ← Range.map]
+        simp only [Function.comp]
+        apply TypeEquivalence.arr (.sum <| .trans _ .listAppR) .refl
+        apply TypeEquivalence.trans (.listApp .refl .listAppL) <| .trans .listAppL <| .list _
+        intro i imem
+        apply TypeEquivalence.app .refl <| .trans .lamAppL _
+        let .list A'opslc := ρ₀ke.soundness Γwe κe.row |>.TypeVarLocallyClosed_of
+        rw [List.map_singleton_flatten] at A'opslc
+        let A''ilc := τ₀ke i imem |>.soundness Γwe κ₀e |>.TypeVarLocallyClosed_of
+        rw [A''ilc.TypeVar_open_eq, A'opslc (A'.Type_open (A'' i)) (Range.mem_map_of_mem imem)
+              |>.weaken (n := 1) |>.Type_open_drop (n := 1) Nat.one_pos |>.TypeVar_open_eq,
+            A''ilc.Type_open_TypeVar_open_eq]
+        exact .refl,
+      .prod_id Alc,
+      .sum_id Alc
+    ⟩
+
+end TabularTypeInterpreter
